Lighter implem of logic conversions

src/language/logic.v
@@ -1,11 +1,13 @@
 Require Import ZArith Psatz.
 Require Import Lists.List.
+Require Import Lists.ListSet.
 Require Import Recdef.
 Require Import Program.Wf.
 Require Import Program.Equality.
 Require Import Logic.FunctionalExtensionality.
 Import ListNotations.
 
+(* Logic language *)
 Inductive logic : Set :=
   | Land  : logic -> logic -> logic
   | Lor   : logic -> logic -> logic
@@ -13,7 +15,129 @@ Inductive logic : Set :=
   | Lneg  : logic -> logic
   | Latom : nat -> logic.
 
-Inductive rule_no_impl : logic -> Prop :=
+(* Logic without impl *)
+Inductive logic_1 : Set :=
+  | L1and   : logic_1 -> logic_1 -> logic_1
+  | L1or    : logic_1 -> logic_1 -> logic_1
+  | L1neg   : logic_1 -> logic_1
+  | L1atom  : nat -> logic_1.
+
+(* Literals *)
+Inductive literal : Set :=
+  | Pos : nat -> literal
+  | Neg : nat -> literal.
+
+(* Logic_1 with distributed negations *)
+Inductive logic_2 : Set :=
+  | L2and   : logic_2 -> logic_2 -> logic_2
+  | L2or    : logic_2 -> logic_2 -> logic_2
+  | L2lit   : literal -> logic_2.
+
+Inductive logic_3 : Set :=.
+
+(* Conversion algorithm from logic to logic_1 *)
+Fixpoint remove_impl (l : logic) : logic_1 :=
+  match l with
+  | Land a b =>
+    L1and (remove_impl a) (remove_impl b)
+  | Lor a b =>
+    L1or (remove_impl a) (remove_impl b)
+  | Limpl a b =>
+    L1or (L1neg (remove_impl a)) (remove_impl b)
+  | Lneg a => L1neg (remove_impl a)
+  | Latom a => L1atom a
+  end.
+
+(* Conversion algorithm from logic_1 to logic_2 *)
+Fixpoint remove_neg' (sign : bool) (l : logic_1) : logic_2 :=
+  match l with
+  | L1and a b =>
+    if sign then L2and (remove_neg' sign a) (remove_neg' sign b)
+    else L2or (remove_neg' false a) (remove_neg' false b)
+  | L1or a b =>
+    if sign then L2or (remove_neg' sign a) (remove_neg' sign b)
+    else L2and (remove_neg' false a) (remove_neg' false b)
+  | L1neg a =>
+    if sign then remove_neg' false a
+    else remove_neg' true a
+  | L1atom n =>
+    if sign then L2lit (Pos n)
+    else L2lit (Neg n)
+  end.
+
+Definition remove_neg := remove_neg' true.
+
+Fixpoint semL (l : logic) (v : nat -> bool) : bool :=
+  match l with
+  | Land a b =>
+    andb (semL a v) (semL b v)
+  | Lor a b =>
+    orb (semL a v) (semL b v)
+  | Limpl a b =>
+    implb (semL a v) (semL b v)
+  | Lneg a =>
+    negb (semL a v)
+  | Latom n => v n
+  end.
+
+Fixpoint semL1 (l : logic_1) (v : nat -> bool) : bool :=
+  match l with
+  | L1and a b =>
+    andb (semL1 a v) (semL1 b v)
+  | L1or a b =>
+    orb (semL1 a v) (semL1 b v)
+  | L1neg a =>
+    negb (semL1 a v)
+  | L1atom n => v n
+  end.
+
+Fixpoint semL2 (l : logic_2) (v : nat -> bool) : bool :=
+  match l with
+  | L2and a b =>
+    andb (semL2 a v) (semL2 b v)
+  | L2or a b =>
+    orb (semL2 a v) (semL2 b v)
+  | L2lit (Pos n) => v n
+  | L2lit (Neg n) => negb (v n)
+  end.
+
+
+Theorem remove_impl_correct:
+  forall l v, semL l v = semL1 (remove_impl l) v.
+Proof.
+  intros.
+  induction l; simpl.
+  - rewrite IHl1, IHl2; reflexivity.
+  - rewrite IHl1, IHl2; reflexivity.
+  - rewrite IHl1, IHl2; unfold implb; destruct semL1; reflexivity.
+  - rewrite IHl; reflexivity.
+  - reflexivity.
+Qed.
+
+Lemma remove_neg_false_negb:
+  forall l v, semL2 (remove_neg' false l) v = negb (semL2 (remove_neg' true l) v).
+Proof.
+  intros.
+  induction l; simpl.
+  - rewrite IHl1, IHl2, Bool.negb_andb; reflexivity.
+  - rewrite IHl1, IHl2, Bool.negb_orb; reflexivity.
+  - rewrite IHl, Bool.negb_involutive; reflexivity.
+  - reflexivity.
+Qed.
+
+Theorem remove_neg_correct:
+  forall l v, semL1 l v = semL2 (remove_neg l) v.
+Proof.
+  intros.
+  induction l; simpl.
+  - rewrite IHl1, IHl2; reflexivity.
+  - rewrite IHl1, IHl2; reflexivity.
+  - rewrite IHl. unfold remove_neg. simpl.
+    rewrite remove_neg_false_negb; reflexivity.
+  - reflexivity.
+Qed.
+
+(* Inductive rule_no_impl : logic -> Prop :=
   | no_impl_and    : forall a b, rule_no_impl a -> rule_no_impl b -> rule_no_impl (Land a b)
   | no_impl_or     : forall a b, rule_no_impl a -> rule_no_impl b -> rule_no_impl (Lor a b)
   | no_impl_neg    : forall a, rule_no_impl a -> rule_no_impl (Lneg a)
@@ -759,4 +883,4 @@ Program Fixpoint distrib_or (l : logic) (P : rule_no_impl l) (Q : rule_no_neg l)
   | Lor a b =>
     Land (distrib_or a _ _) (distrib_or b _ _)
   end.
-  
+   *)
